Move [naive_blit] to the attic.

src/array.v
@@ -865,28 +865,6 @@ Context `{Inhabited A}.
 Implicit Types a b : array A.
 Implicit Types xs ys : list A.
 
-(* The code. *)
-
-Section Code.
-Open Scope uint63.
-
-(* We begin with a naive definition, using [iter_up] so as to save
-   the trouble of writing a loop. *)
-
-(* We compute [_delta] outside of the loop so as to save one addition
-   inside the loop. This is a bit subtle, as the difference [_j - _i]
-   might be negative, yet we compute it as an unsigned integer. This
-   yields the correct result in the end anyway. *)
-
-Definition naive_blit a _i b _j _n :=
-  do _delta ← _j - _i ;
-  iter_up _i (_i + _n) b @@ λ _k b,
-  do x ← get a _k ;
-  do b ← set b (_k + _delta) x ;
-  b.
-
-End Code.
-
 (* The postcondition of a [blit] function. *)
 
 Notation blit_post xs i ys j n := (
@@ -910,35 +888,8 @@ Definition blit_spec (blit : array A → int → array A → int → array A) n 
   valid_seg j (j + n) ys →
   wp (blit a _i b _j) (blit_post xs i ys j n).
 
-(* [naive_blit] is correct. *)
-
-Lemma wp_naive_blit :
-  ∀Int _n n,
-  blit_spec (λ a _i b _j, naive_blit a _i b _j _n) n.
-Proof.
-  unfold blit_spec, naive_blit. intros. arrays.
-  wp_bind_eq.
-  wp_op wp_iter_up with invariant: (λ k, blit_post xs i ys j (k - i));
-  last wp_shadow b.
-  (* Initialization. *)
-  { isArray. }
-  (* Preservation. *)
-  { clear dependent b. wp_iter_up_body _k k b.
-    wp_get x. subst x.
-    (* The use of unsigned arithmetic in the computation of [_delta]
-       does not cause any problem. Once upon a time, this proof used
-       natural numbers as the logical model of machine integers; then
-       we had to explicitly say [rewrite int.add_sub_exch] in order to
-       pretend that we never created a negative number. Now this trick
-       is unnecessary. *)
-    wp_set. wp_ret. isArray. }
-  (* Completion. *)
-  { isArray. }
-Qed.
-
-(* We continue with a second naive [blit] function. The algorithm is
-   essentially the same (it is just a loop). This time we do not use
-   the higher-order function [iter_up]. Thus we hope to save the cost
+(* We begin with a simple [blit] function. Although we could, we do not
+   use the higher-order function [iter_up]. Thus we hope to save the cost
    of using a higher-order iteration function. *)
 
 (* We use a formulation as a tail-recursive function where the parameter
