attic/naive_blit.v
@@ -1,0 +1,45 @@
+Section Code.
+Open Scope uint63.
+
+(* We begin with a naive definition, using [iter_up] so as to save
+   the trouble of writing a loop. *)
+
+(* We compute [_delta] outside of the loop so as to save one addition
+   inside the loop. This is a bit subtle, as the difference [_j - _i]
+   might be negative, yet we compute it as an unsigned integer. This
+   yields the correct result in the end anyway. *)
+
+Definition naive_blit a _i b _j _n :=
+  do _delta ← _j - _i ;
+  iter_up _i (_i + _n) b @@ λ _k b,
+  do x ← get a _k ;
+  do b ← set b (_k + _delta) x ;
+  b.
+
+End Code.
+
+(* [naive_blit] is correct. *)
+
+Lemma wp_naive_blit :
+  ∀Int _n n,
+  blit_spec (λ a _i b _j, naive_blit a _i b _j _n) n.
+Proof.
+  unfold blit_spec, naive_blit. intros. arrays.
+  wp_bind_eq.
+  wp_op wp_iter_up with invariant: (λ k, blit_post xs i ys j (k - i));
+  last wp_shadow b.
+  (* Initialization. *)
+  { isArray. }
+  (* Preservation. *)
+  { clear dependent b. wp_iter_up_body _k k b.
+    wp_get x. subst x.
+    (* The use of unsigned arithmetic in the computation of [_delta]
+       does not cause any problem. Once upon a time, this proof used
+       natural numbers as the logical model of machine integers; then
+       we had to explicitly say [rewrite int.add_sub_exch] in order to
+       pretend that we never created a negative number. Now this trick
+       is unnecessary. *)
+    wp_set. wp_ret. isArray. }
+  (* Completion. *)
+  { isArray. }
+Qed.
